\documentclass{article}
\usepackage{ifthen}
\usepackage{epsfig}
\usepackage[utf8]{inputenc}
% Packages requested by user
\usepackage{tikz}
\usepackage{circuitikz}

\usepackage{newunicodechar}
  \newunicodechar{⁻}{${}^{-}$}% Superscript minus
  \newunicodechar{²}{${}^{2}$}% Superscript two
  \newunicodechar{³}{${}^{3}$}% Superscript three

\pagestyle{empty}
\begin{document}
\[ \mathbf{E}(\mathbf{y}, t) \cdot \dot{\mathbf{y}}+\mathbf{F}(\mathbf{y}, t) \cdot \mathbf{y}+\mathbf{c}(\mathbf{y}, t)=\mathbf{0} \]
\pagebreak

$y$
\pagebreak

$\dot{y}$
\pagebreak

$N$
\pagebreak

$\alpha$
\pagebreak

\[ [P_{in}^1, Q_{in}^1, \dots, P_{in}^n, Q_{in}^n, P_{out}^1, Q_{out}^1, \dots, P_{out}^m, Q_{out}^m, V^{1}, \dots, V^{p}] \]
\pagebreak

$P_{in} $
\pagebreak

$Q_{in} $
\pagebreak

$P_{out} $
\pagebreak

$Q_{out} $
\pagebreak

$V $
\pagebreak

\[ \begin{circuitikz} \draw node[left] {$Q_{in}$} [-latex] (0,0) -- (0.8,0); \draw (1,0) node[anchor=south]{$P_{in}$} to [R, l=$R$, *-] (3,0) to [L, l=$L$, *-*] (5,0) node[anchor=south]{$P_{out}$} (3,0) to [C, l=$C$, *-] (3,-1.5) node[ground]{$P_C$}; \draw [-latex] (5.2,0) -- (6,0) node[right] {$Q_{out}$}; \end{circuitikz} \]
\pagebreak

\[ P_{in}^{e}-P_{out}^{e}-R Q_{in}^{e}-L\frac{d Q_{out}^{e}}{dt}=0 \]
\pagebreak

\[ Q_{i n}^{e}-Q_{o u t}^{e}-C \frac{d P_{c}^{e}}{d t}=0 \]
\pagebreak

\[ P_{i n}^{e}-R Q_{i n}^{e}-P_{c}=0 \]
\pagebreak

\[ \mathbf{y}^{e}=\left[\begin{array}{lllll}P_{i n}^{e} & Q_{in}^{e} & P_{out}^{e} & Q_{out}^{e} & P_C\end{array}\right]^{T} \]
\pagebreak

\[ \mathbf{E}^{e}=\left[\begin{array}{ccccc} 0 & 0 & 0 & -L & 0 \\ 0 & 0 & 0 & 0 & -C \\ 0 & 0 & 0 & 0 & 0 \end{array}\right] \]
\pagebreak

\[ \mathbf{F}^{e}=\left[\begin{array}{ccccc} 1 & -R_{ste}-R & -1 & 0 & 0 \\ 0 & 1 & 0 & -1 & 0 \\ 1 & -R_{ste}-R & 0 & 0 & -1 \end{array}\right] \]
\pagebreak

\[ \mathbf{D}^{e}=\left[\begin{array}{ccccc} 0 & -R_{ste} & 0 & 0 & 0 \\ 0 & 0 & 0 & 0 & 0 \\ 0 & -R_{ste} & 0 & 0 & 0 \end{array}\right] \]
\pagebreak

$ R_{ste}=K_{t} \frac{\rho}{2 A_{o}^{2}}\left(\frac{A_{o}}{A_{s}}-1\right)^{2}|Q_{in}^{e}| $
\pagebreak

$R$
\pagebreak

$C$
\pagebreak

$L$
\pagebreak

\[ \begin{circuitikz} \draw node[left] {$\hat{Q}$} [-latex] (0,0) -- (0.8,0); \draw (1,0) node[anchor=south]{$P$} to [short, *-] (1.2,0) ; \draw [-latex] (1.4,0) -- (2.2,0) node[right] {$Q$}; \end{circuitikz} \]
\pagebreak

\[ Q=\hat{Q} \]
\pagebreak

\[ \mathbf{y}^{e}=\left[\begin{array}{ll}P^{e} & Q^{e}\end{array}\right]^{T} \]
\pagebreak

\[ \mathbf{F}^{e}=\left[\begin{array}{ll}0 & 1\end{array}\right] \]
\pagebreak

\[ \mathbf{C}^{e}=\left[\hat{Q}\right] \]
\pagebreak

\[ \begin{circuitikz} \draw node[left] {$Q_{in}$} [-latex] (0,0) -- (0.8,0); \draw (1,0) node[anchor=south]{$P_{in}$} to [short, *-*] (3.0,0); \draw (3,0) node[anchor=south]{} to [short, -*] (4.5,1.0); \draw (4.3,1.1) node[anchor=south] {$P_{out,1}$}; \draw (3,0) node[anchor=south]{} to [short, -*] (4.5,-1.0); \draw (4.3,-1.1) node[anchor=north] {$P_{out,2}$}; \draw [-latex] (4.65,1.1) -- (5.25,1.5) node[right] {$Q_{out,1}$}; \draw [-latex] (4.65,-1.1) -- (5.25,-1.5) node[right] {$Q_{out,2}$}; \end{circuitikz} \]
\pagebreak

\[ \sum_{i}^{n_{inlets}} Q_{in, i}=\sum_{j}^{n_{outlets}} Q_{out, j} \]
\pagebreak

\[ P_{i}=P_{j} \quad \mathrm{with} \quad i \neq j \]
\pagebreak

\[ \mathbf{y}^{e}=\left[\begin{array}{llllllllll}P_{in, 1}^{e} & Q_{in, 1}^{e} & \dots & P_{in, i}^{e} & Q_{in, i}^{e} & P_{out, 1}^{e} & Q_{out, 1}^{e} & \dots & P_{out, i}^{e} & Q_{out, i}^{e}\end{array}\right] \]
\pagebreak

\[ \mathbf{F}^{e}_1 = \left[\begin{array}{llllllllll}0 & 1 & 0 & 1 & \dots & 0 & -1 & 0 & -1 & \dots\end{array}\right] \]
\pagebreak

\[ \mathbf{F}^{e}_{2,...,n} = \left[\begin{array}{lllll}\dots & \underbrace{1}_{P_i} & \dots & \underbrace{1}_{P_j} & \dots\end{array}\right] \quad \mathrm{with} \quad i \neq j \]
\pagebreak

\[ \begin{circuitikz} \draw node[left] {$Q_{in}$} [-latex] (0,0) -- (0.8,0); \draw (1,0) node[anchor=south]{$P_{in}$} to [R, l=$R_p$, *-] (3,0) to [R, l=$R_d$, *-*] (5,0) node[anchor=south]{$P_{ref}$} (3,0) to [C, l=$C$, *-] (3,-1.5) node[ground]{$P_{C}$}; \end{circuitikz} \]
\pagebreak

\[ R_{d} Q^{e}-P_{c}^{e}+P_{r e f}-R_{d} C \frac{d P_{c}^{e}}{d t}=0 \]
\pagebreak

\[ P^{e}-P_{c}^{e}-R_{p} Q^{e}=0 \]
\pagebreak

\[ \mathbf{y}^{e}=\left[\begin{array}{lll}P^{e} & Q^{e} & P_{c}^{e}\end{array}\right]^{T} \]
\pagebreak

\[ \mathbf{E}^{e}=\left[\begin{array}{ccc} 0 & 0 & -R_{d} C \\ 0 & 0 & 0 \end{array}\right] \]
\pagebreak

\[ \mathbf{F}^{e}=\left[\begin{array}{ccc} 0 & R_{d} & -1 \\ 1 & -R_{p} & -1 \end{array}\right] \]
\pagebreak

\[ \mathbf{c}^{e}=\left[\begin{array}{c} P_{r e f} \\ 0 \end{array}\right] \]
\pagebreak

\end{document}
